# RDFStats configuration vocabulary

@prefix rdfs:   <http://www.w3.org/2000/01/rdf-schema#> .
@prefix rdf:    <http://www.w3.org/1999/02/22-rdf-syntax-ns#> .
@prefix xsd:    <http://www.w3.org/2001/XMLSchema#> .
@prefix ja:     <http://jena.hpl.hp.com/2005/11/Assembler#> .
@prefix :		<http://purl.org/rdfstats/config#> .


### MEDIATOR CONFIGURATION ######################################

:Configuration		a rdfs:Class ;
	rdfs:comment	"Configuration of the RDFStats Generator" .

:histogramSize 		a rdf:Property ;
	rdfs:comment	"Preferred number of absolute bins" ;
	rdfs:domain		:Configuration ;
	rdfs:range		xsd:integer .

:statsModel			a rdf:Property ;
	rdfs:comment	"A Jena Assembler model - the target model where to store the created statistics" ;
	rdfs:domain		:Configuration ;
	rdfs:range		ja:Model .

:outputFile			a rdf:Property ;
	rdfs:comment	"The output file (local filename) - if specified, :statsModel will be ignored!" ;
	rdfs:domain		:Configuration ;
	rdfs:range		xsd:string .

:outputFormat		a rdf:Property ;
	rdfs:comment	"The output format to use when saving the results to a file (Jena-style: 'RDF/XML', 'N3', or 'N-TRIPLES'), default is 'N3'" ;
	rdfs:domain		:Configuration ;
	rdfs:range		xsd:string .

:endpointUri		a rdf:Property ;
	rdfs:comment	"A SPARQL end-point to process (multiple values allowed)" ;
	rdfs:domain		:Configuration ;
	rdfs:range		rdfs:Resource .

:documentUrl		a rdf:Property ;
	rdfs:comment	"An RDF document source URL (may be file:... or http://... etc.)" ;
	rdfs:domain		:Configuration ;
	rdfs:range		rdfs:Resource .

:stringHistMaxLength	a rdf:Property ;
	rdfs:comment	"Maximal length of strings processed for StringOrderedHistogram" ;
	rdfs:domain		:Configuration ;
	rdfs:range		xsd:integer .

:quickMode			a rdf:Property ;
	rdfs:comment	"Quick mode: only generate histograms for new classes or if the number of total instances has changed from previous statistics" ;
	rdfs:domain		:Configuration ;
	rdfs:range		xsd:boolean .

:defaultTimezone	a rdf:Property ;
	rdfs:comment	"Time zone to use for dates which have no time zone information (a string value as defined in http://java.sun.com/j2se/1.5.0/docs/api/java/util/TimeZone.html)." ;
	rdfs:domain		:Configuration ;
	rdfs:range		xsd:string .

# deprecated
#:classSpecificHistograms	a rdf:Property ;
#	rdfs:comment	"Create class-specific histograms" ;
#	rdfs:domain		:Configuration ;
#	rdfs:range		xsd:boolean .
